prog draft finished

src/sequentialization/Programs.v
@@ -2,6 +2,7 @@ From hahn Require Import Hahn.
 From hahnExt Require Import HahnExt.
 From imm Require Import Events Execution.
 From xmm Require Import Instructions.
+From xmm Require Import Core.
 Require Import Lia Setoid Program.Basics.
 Require Import Coq.Sorting.Mergesort.
 Require Import Coq.Structures.OrderedType.
@@ -11,7 +12,35 @@ Open Scope program_scope.
 
 Section Program.
 
-Definition state : Set := location -> value.
+Definition program_trace := thread_id -> list label.
+Definition program := program_trace -> Prop.
+
+Record program_trace_sequented (p_tr1 p_tr2 : program_trace) (t1 t2 : thread_id) : Prop :=
+    { p_tr_eq : forall t, t <> t1 /\ t <> t2 -> p_tr1 t = p_tr2 t;
+      p_tr_empty : p_tr2 t2 = [];
+      p_tr_concat : p_tr2 t1 = p_tr1 t1 ++ p_tr1 t2;
+    }. 
+
+Definition corresp_px (exec : WCore.t) (p_tr : program_trace) : Prop :=
+    forall t i, (acts_set (WCore.G exec)) (ThreadEvent t i) -> 
+            Some (lab (WCore.G exec) (ThreadEvent t i)) = nth_error (p_tr t) i.
+
+Definition program_sequented (p1 p2 : program) (t1 t2 : thread_id) : Prop :=
+    forall p_tr : program_trace,
+        p2 p_tr -> exists p_tr', p1 p_tr' /\ 
+        program_trace_sequented p_tr' p_tr t1 t2.
+
+Record exec_sequent (ex1 ex2 : WCore.t) (p1 p2 : program)
+                        (t1 t2 : thread_id) : Prop := {
+    exec_sequented : program_sequented p1 p2 t1 t2;
+    traces_cond : forall p_tr1 p_tr2 : program_trace,
+        p1 p_tr1 -> p2 p_tr2 ->
+        corresp_px ex1 p_tr1 ->
+        corresp_px ex2 p_tr2 ->
+        program_trace_sequented p_tr1 p_tr2 t1 t2;
+    }.
+
+(* Definition state : Set := location -> value.
 Definition prog_threads : Set := nat.
 Definition state_init := prog_threads -> state.
 
@@ -102,8 +131,6 @@ Definition trace_conforming_thread (prog : program) (t : thread_id) (N : nat) : 
       is_subsequence (thread_events_labs (thread_event_list t N)) (extract_labels_from_program prog).
 
 Definition trace_conforming (prog : program) (N : nat) : Prop :=
-    forall t, trace_conforming_thread prog t N.
-
-
+    forall t, trace_conforming_thread prog t N. *)
 
 End Program.
