src/sequentialization/Sequent.v
@@ -9,6 +9,7 @@ Require Import xmm_s_hb.
 Require Import Lia.
 From xmm Require Import Reordering.
 From xmm Require Import ThreadTrace.
+From xmm Require Import Programs.
 
 From hahn Require Import Hahn.
 From hahnExt Require Import HahnExt.
@@ -142,6 +143,7 @@ Section SimrelStep.
 Variable X_t X_t' X_s : WCore.t.
 Variable t_1 t_2 : thread_id.
 Variable mapper : actid -> actid.
+Variable mapper_rev : actid -> actid.
 
 Variable e : actid.
 Variable l : label.
@@ -217,8 +219,10 @@ Notation "'F_s'" := (F G_s).
 
 Notation "'Tid_' t" := (fun e => tid e = t) (at level 1).
 
-Lemma simrel_step_e
-    (n : nat)
+Hypothesis MAPREV : eq_dom E_t (mapper_rev ∘ mapper) id.
+
+Lemma simrel_step_e_t1 (n : nat)
+    (T1 : tid e = t_1) (IND: index e < n)
     (NINIT1 : t_1 <> tid_init)
     (NINIT2 : t_2 <> tid_init)
     (T2NOTIN : ~ threads_set G_t t_2)
@@ -233,317 +237,335 @@ Lemma simrel_step_e
 Proof using.
   destruct STEP as [ADD RFC CONS].
   destruct ADD as (r & R1 & w & W1 & W2 & ADD).
+  set (mapper' := upd mapper e e).
+  set (mapper_rev' := upd mapper_rev e e).
+  assert (ENOTIN : ~E_t e) by apply ADD.
+  assert (MAPEQ : eq_dom E_t mapper' mapper).
+  { subst mapper'. unfolder. intros x XINE.
+    clear - ENOTIN XINE. rewrite updo.
+    all: congruence. }
+  assert (MAPER_E : mapper' ↑₁ eq e ≡₁ eq e).
+  { subst mapper'. rewrite set_collect_eq. now rupd. }
+  assert (MAPSUB : mapper' ↑₁ E_t ≡₁ mapper ↑₁ E_t).
+  { clear - MAPEQ. now apply set_collect_eq_dom. }
+  assert (EQACTS : E_t' ≡₁ E_t ∪₁ eq e) by apply ADD.
+  assert (NEWE :
+  << NINIT : ~is_init e >> /\
+  << NOTIN : ~E_s e >> /\
+  << TID : tid e = t_1 >>). 
+  (* /\
+  << NEWSB : ⦗E_s ∪₁ eq e⦘ ⨾ ext_sb ⨾ ⦗E_s ∪₁ eq e⦘ ≡
+          sb_s ∪ WCore.sb_delta e E_s >>). *)
+  { unfold NW; splits; vauto.
+    { intro FALSO. unfold is_init in FALSO. desf. }
+    admit. }
+  (*  { unfold sb.
+      rewrite (rsr_actsE CORR SIMREL).
+      unfold extra_a; desf; [exfalso; now apply ETID|].
+      rewrite set_union_empty_r.
+      rewrite <- EQACTS. apply ADD. }
+    unfold sb.
+    rewrite rsr_actsE
+      with (X_s := X_s) (X_t := X_t)
+          (a_t := a_t) (b_t := b_t); eauto.
+    unfold extra_a; desf.
+    { rewrite <- (rsr_at_bt_tid CORR) in NQT.
+      rewrite id_union, !seq_union_l, !seq_union_r.
+      arewrite_false (⦗eq e⦘ ⨾ ext_sb ⨾ ⦗eq e⦘).
+      { clear. unfolder. ins. desf.
+        eapply ext_sb_irr; eauto. }
+      arewrite_false (⦗eq e⦘ ⨾ ext_sb ⨾ ⦗E_t ∪₁ eq a_t⦘).
+      { admit. }
+      rewrite id_union at 3. rewrite seq_union_l.
+      arewrite_false (⦗eq a_t⦘ ⨾ ext_sb ⨾ ⦗eq e⦘).
+      { clear - NQT CORR. unfolder. unfold ext_sb.
+        ins. desf; ins; [| desf].
+        apply (rsr_at_ninit CORR). auto. }
+      rewrite sb_delta_union.
+      assert (SUB : WCore.sb_delta e (eq a_t) ⊆ WCore.sb_delta e E_t).
+      { clear - NQT. unfolder. ins. desf. auto. }
+      rewrite union_absorb_r with (r := WCore.sb_delta e (eq a_t)); auto.
+      rewrite !union_false_r. apply union_more; [reflexivity |].
+      arewrite (⦗E_t⦘ ⨾ ext_sb ⨾ ⦗eq e⦘ ≡ ⦗E_t⦘ ⨾ sb_t' ⨾ ⦗eq e⦘).
+      { unfold sb. rewrite !seqA. seq_rewrite <- !id_inter.
+        rewrite EQACTS. clear - ENOTIN. basic_solver 11. }
+      rewrite (WCore.add_event_sb ADD), seq_union_l.
+      arewrite_false (sb_t ⨾ ⦗eq e⦘).
+      { clear - ENOTIN. rewrite wf_sbE. basic_solver. }
+      rewrite union_false_l. unfold WCore.sb_delta.
+      seq_rewrite <- cross_inter_l.
+      rewrite set_inter_union_r, 2!set_inter_absorb_l.
+      all: try now apply CORR.
+      all: basic_solver 11. }
+    rewrite !set_union_empty_r.
+    rewrite <- EQACTS. apply ADD. } *)
+  unfold NW in NEWE.
+  destruct NEWE as (NINIT & NOTIN & TID).
 
-  destruct classic with (tid e = t_1) as [TIDE | TIDE].
-  { destruct classic with (index e < n) as [LQ | BQ].
-    {
-      set (mapper' := upd mapper e e).
+  set (G_s' := {|
+  acts_set := mapper' ↑₁ E_t';
+    threads_set := threads_set G_s;
+    lab := lab_t' ∘ mapper_rev';
+    rf := mapper' ↑ rf_t';
+    co := mapper' ↑ co_t';
+    rmw := mapper' ↑ rmw_t';
+    rmw_dep := rmw_dep_t';
+    ctrl := ctrl_t';
+    data := data_t';
+    addr := addr_t';
+  |}).
+  set (X_s' := {|
+    WCore.sc := WCore.sc X_s;
+    WCore.G := G_s';
+  |}).
 
-      assert (ENOTIN : ~E_t e) by apply ADD.
-      assert (MAPEQ : eq_dom E_t mapper' mapper).
-      { subst mapper'. unfolder. intros x XINE.
-        clear - ENOTIN XINE. rewrite updo.
-        all: congruence. }
-      assert (MAPER_E : mapper' ↑₁ eq e ≡₁ eq e).
-      { subst mapper'. rewrite set_collect_eq. now rupd. }
-      assert (MAPSUB : mapper' ↑₁ E_t ≡₁ mapper ↑₁ E_t).
-      { clear - MAPEQ. now apply set_collect_eq_dom. }
-      assert (EQACTS : E_t' ≡₁ E_t ∪₁ eq e) by apply ADD.
-
-      assert (NEWE :
-      << NINIT : ~is_init e >> /\
-      << NOTIN : ~E_s e >> /\
-      << TID : tid e = t_1 >>). 
-      (* /\
-      << NEWSB : ⦗E_s ∪₁ eq e⦘ ⨾ ext_sb ⨾ ⦗E_s ∪₁ eq e⦘ ≡
-              sb_s ∪ WCore.sb_delta e E_s >>). *)
-      { unfold NW; splits; vauto.
-        { intro FALSO. unfold is_init in FALSO. desf. }
+  exists mapper', X_s'.
+  assert (MAPPINV' : eq_dom E_t' (mapper' ∘ mapper') id).
+  { unfold mapper'. unfold eq_dom. intros x XINE. 
+    destruct classic with (x = e) as [EQ | NEQ].
+    { subst x. unfold compose. rewrite !upds; vauto. }
+    unfold compose. rewrite !updo; vauto.
+    assert (NINE : E_t x).
+    { apply EQACTS in XINE.
+      destruct XINE as [XINE | XINE]; vauto. }
+    { apply MAPINV; vauto. }
+    rewrite updo; vauto.
+    intros FALSE.
+    assert (INE : E_s (mapper x)).
+    { apply SIMREL. unfold set_collect.
+      exists x; split.
+      { apply EQACTS in XINE. 
+        clear - XINE NEQ. destruct XINE; basic_solver. }
+      vauto. }
+    basic_solver. }
+  splits; vauto.
+  { constructor; vauto; simpl; try basic_solver 6.
+    { rewrite (WCore.add_event_acts ADD). apply inj_dom_union.
+      { clear - SIMREL MAPEQ.
+        unfolder. ins. apply (seq_inj SIMREL); ins.
+        now rewrite <- !MAPEQ. }
+      { clear. basic_solver. }
+      rewrite MAPER_E, MAPSUB, (seq_codom SIMREL).
+      clear - NOTIN. basic_solver. }
+    { intros ev INE' TIDCOND.
+      destruct classic with (ev = e) as [EQ | NEQ].
+      { subst ev. unfold mapper'. rewrite upds; vauto. }
+      unfold mapper'. rewrite updo; vauto.
+      apply (seq_tid_1 SIMREL); vauto.
+      apply EQACTS in INE'. destruct INE' as [C1 | C2]; vauto.
+      unfold mapper' in TIDCOND. rewrite updo in TIDCOND; vauto. }
+    { intros ev INE' TIDCOND.
+      destruct classic with (ev = e) as [EQ | NEQ]; vauto.
+      apply (seq_tid_2 SIMREL); vauto.
+      { apply EQACTS in INE'. destruct INE' as [C1 | C2]; vauto. }
+      unfold mapper'. rewrite updo; vauto. }
+    { intros x COND. unfold compose.
+      destruct classic with (x = e) as [EQ | NEQ].
+      { subst x. unfold mapper', mapper_rev'.
+        rewrite !upds; vauto. }
+      unfold mapper', mapper_rev'.
+      rewrite !updo; vauto.
+      { unfold compose in MAPREV. rewrite MAPREV.
         admit. }
-        
-        
-      (*  { unfold sb.
-          rewrite (rsr_actsE CORR SIMREL).
-          unfold extra_a; desf; [exfalso; now apply ETID|].
-          rewrite set_union_empty_r.
-          rewrite <- EQACTS. apply ADD. }
-        unfold sb.
-        rewrite rsr_actsE
-          with (X_s := X_s) (X_t := X_t)
-              (a_t := a_t) (b_t := b_t); eauto.
-        unfold extra_a; desf.
-        { rewrite <- (rsr_at_bt_tid CORR) in NQT.
-          rewrite id_union, !seq_union_l, !seq_union_r.
-          arewrite_false (⦗eq e⦘ ⨾ ext_sb ⨾ ⦗eq e⦘).
-          { clear. unfolder. ins. desf.
-            eapply ext_sb_irr; eauto. }
-          arewrite_false (⦗eq e⦘ ⨾ ext_sb ⨾ ⦗E_t ∪₁ eq a_t⦘).
-          { admit. }
-          rewrite id_union at 3. rewrite seq_union_l.
-          arewrite_false (⦗eq a_t⦘ ⨾ ext_sb ⨾ ⦗eq e⦘).
-          { clear - NQT CORR. unfolder. unfold ext_sb.
-            ins. desf; ins; [| desf].
-            apply (rsr_at_ninit CORR). auto. }
-          rewrite sb_delta_union.
-          assert (SUB : WCore.sb_delta e (eq a_t) ⊆ WCore.sb_delta e E_t).
-          { clear - NQT. unfolder. ins. desf. auto. }
-          rewrite union_absorb_r with (r := WCore.sb_delta e (eq a_t)); auto.
-          rewrite !union_false_r. apply union_more; [reflexivity |].
-          arewrite (⦗E_t⦘ ⨾ ext_sb ⨾ ⦗eq e⦘ ≡ ⦗E_t⦘ ⨾ sb_t' ⨾ ⦗eq e⦘).
-          { unfold sb. rewrite !seqA. seq_rewrite <- !id_inter.
-            rewrite EQACTS. clear - ENOTIN. basic_solver 11. }
-          rewrite (WCore.add_event_sb ADD), seq_union_l.
-          arewrite_false (sb_t ⨾ ⦗eq e⦘).
-          { clear - ENOTIN. rewrite wf_sbE. basic_solver. }
-          rewrite union_false_l. unfold WCore.sb_delta.
-          seq_rewrite <- cross_inter_l.
-          rewrite set_inter_union_r, 2!set_inter_absorb_l.
-          all: try now apply CORR.
-          all: basic_solver 11. }
-        rewrite !set_union_empty_r.
-        rewrite <- EQACTS. apply ADD. } *)
-      unfold NW in NEWE.
-      destruct NEWE as (NINIT & NOTIN & TID).
+      admit. }
+    { admit. (*TODO : po-work*) }
+    { rewrite (seq_threads SIMREL).
+      destruct ADD. rewrite add_event_threads; vauto. }
+    unfold mapper'. intros x COND.
+    destruct classic with (x = e) as [EQ | NEQ].
+    { subst x. rewrite upds; vauto. }
+    rewrite updo; vauto.
+    apply (seq_init SIMREL); vauto. }
+  constructor.
+  { unfold WCore.add_event.
+    exists (option_map mapper' r), (mapper' ↑₁ R1),
+        (option_map mapper' w),
+        (mapper' ↑₁ W1),
+        (mapper' ↑₁ W2).
+    apply add_event_to_wf; simpl; vauto.
+    { apply sico_init_acts_s with
+            (X_t := X_t) (mapper := mapper).
+      { constructor. all : apply SIMREL. }
+      destruct ADD. apply add_event_init. }
+    { unfold mapper'. rewrite upds. exact NOTIN. }
+    { unfold mapper'. rewrite upds; vauto. }
+    { unfold mapper'. rewrite upds. basic_solver. }
+    { rewrite EQACTS. rewrite set_collect_union.
+      rewrite MAPER_E, MAPSUB. rewrite (seq_acts SIMREL).
+      unfold mapper'. rewrite upds. basic_solver. }
+    { unfold mapper'.
+      destruct ADD. rewrite add_event_lab.
+      unfold compose. rewrite upds.
+      admit. }
+    all : admit. }
+  all : admit.
+Admitted.
 
-      set (G_s' := {|
-      acts_set := mapper' ↑₁ E_t';
-        threads_set := threads_set G_s;
-        lab := lab_t' ∘ mapper';
-        rf := mapper' ↑ rf_t';
-        co := mapper' ↑ co_t';
-        rmw := mapper' ↑ rmw_t';
-        rmw_dep := rmw_dep_t';
-        ctrl := ctrl_t';
-        data := data_t';
-        addr := addr_t';
-      |}).
-      set (X_s' := {|
-        WCore.sc := WCore.sc X_s;
-        WCore.G := G_s';
-      |}).
+Lemma simrel_step_e_t2 (n : nat)
+    (T1 : tid e = t_1) (IND: index e >= n)
+    (NINIT1 : t_1 <> tid_init)
+    (NINIT2 : t_2 <> tid_init)
+    (T2NOTIN : ~ threads_set G_t t_2)
+    (THRDNEQ : t_1 <> t_2)
+    (SIMREL : seq_simrel X_s X_t t_1 t_2 mapper)
+    (STEP : WCore.exec_inst X_t X_t' e l)
+    (MAPINV : eq_dom E_t (mapper ∘ mapper) id) :
+  exists mapper' X_s',
+    << MAPINV' : eq_dom E_t' (mapper' ∘ mapper') id >> /\
+    << SIMREL : seq_simrel X_s' X_t' t_1 t_2 mapper' >> /\
+    << STEP : WCore.exec_inst X_s X_s' (mapper' e) l >>.
+Proof using.
+  destruct STEP as [ADD RFC CONS].
+  destruct ADD as (r & R1 & w & W1 & W2 & ADD).
+  set (mapper' := upd mapper e (ThreadEvent t_2 (index e - n))).
+  assert (ENOTIN : ~E_t e) by apply ADD.
+  assert (MAPEQ : eq_dom E_t mapper' mapper).
+  { subst mapper'. unfolder. intros x XINE.
+    clear - ENOTIN XINE. rewrite updo.
+    all: congruence. }
+  assert (MAPER_E : mapper' ↑₁ eq e ≡₁ eq (ThreadEvent t_2 (index e - n))).
+  { subst mapper'. rewrite set_collect_eq. now rupd. }
+  assert (MAPSUB : mapper' ↑₁ E_t ≡₁ mapper ↑₁ E_t).
+  { clear - MAPEQ. now apply set_collect_eq_dom. }
+  assert (EQACTS : E_t' ≡₁ E_t ∪₁ eq e) by apply ADD.
+  assert (NEWE :
+    << NINIT : ~is_init e >> /\
+    << NOTIN : ~E_s e >> /\
+    << TID : tid e = t_1 >>). 
+  { admit. }
+  unfold NW in NEWE. destruct NEWE as (NINIT & NOTIN & TID).
 
-      exists mapper', X_s'.
-      assert (MAPPINV' : eq_dom E_t' (mapper' ∘ mapper') id).
-      { unfold mapper'. unfold eq_dom. intros x XINE. 
-        destruct classic with (x = e) as [EQ | NEQ].
-        { subst x. unfold compose. rewrite !upds; vauto. }
-        unfold compose. rewrite !updo; vauto.
-        assert (NINE : E_t x).
-        { apply EQACTS in XINE.
-          destruct XINE as [XINE | XINE]; vauto. }
-        { apply MAPINV; vauto. }
-        rewrite updo; vauto.
-        intros FALSE.
-        assert (INE : E_s (mapper x)).
-        { apply SIMREL. unfold set_collect.
-          exists x; split.
-          { apply EQACTS in XINE. 
-            clear - XINE NEQ. destruct XINE; basic_solver. }
-          vauto. }
-        basic_solver. }
-      splits; vauto.
-      { constructor; vauto; simpl; try basic_solver 6.
-        { rewrite (WCore.add_event_acts ADD). apply inj_dom_union.
-          { clear - SIMREL MAPEQ.
-            unfolder. ins. apply (seq_inj SIMREL); ins.
-            now rewrite <- !MAPEQ. }
-          { clear. basic_solver. }
-          rewrite MAPER_E, MAPSUB, (seq_codom SIMREL).
-          clear - NOTIN. basic_solver. }
-        { intros ev INE' TIDCOND.
-          destruct classic with (ev = e) as [EQ | NEQ].
-          { subst ev. unfold mapper'. rewrite upds; vauto. }
-          unfold mapper'. rewrite updo; vauto.
-          apply (seq_tid_1 SIMREL); vauto.
-          apply EQACTS in INE'. destruct INE' as [C1 | C2]; vauto.
-          unfold mapper' in TIDCOND. rewrite updo in TIDCOND; vauto. }
-        { intros ev INE' TIDCOND.
-          destruct classic with (ev = e) as [EQ | NEQ]; vauto.
-          apply (seq_tid_2 SIMREL); vauto.
-          { apply EQACTS in INE'. destruct INE' as [C1 | C2]; vauto. }
-          unfold mapper'. rewrite updo; vauto. }
-        { intros x COND. unfold compose.
-          arewrite (mapper' (mapper' x) = x); vauto. }
-        { admit. (*TODO : po-work*) }
-        { rewrite (seq_threads SIMREL).
-          destruct ADD. rewrite add_event_threads; vauto. }
-        unfold mapper'. intros x COND.
-        destruct classic with (x = e) as [EQ | NEQ].
-        { subst x. rewrite upds; vauto. }
-        rewrite updo; vauto.
-        apply (seq_init SIMREL); vauto. }
-      constructor.
-      { unfold WCore.add_event.
-        exists (option_map mapper' r), (mapper' ↑₁ R1),
-            (option_map mapper' w),
-            (mapper' ↑₁ W1),
-            (mapper' ↑₁ W2).
-        apply add_event_to_wf; simpl; vauto.
-        { apply sico_init_acts_s with
-                (X_t := X_t) (mapper := mapper).
-          { constructor. all : apply SIMREL. }
-          destruct ADD. apply add_event_init. }
-        { unfold mapper'. rewrite upds. exact NOTIN. }
-        { unfold mapper'. rewrite upds; vauto. }
-        { unfold mapper'. rewrite upds. basic_solver. }
-        { rewrite EQACTS. rewrite set_collect_union.
-          rewrite MAPER_E, MAPSUB. rewrite (seq_acts SIMREL).
-          unfold mapper'. rewrite upds. basic_solver. }
-        { unfold mapper'.
-          destruct ADD. rewrite add_event_lab.
-          unfold compose. rewrite upds.
-          admit. }
-        all : admit. }
-      all : admit. }
-    { set (mapper' := upd mapper e (ThreadEvent t_2 (index e - n))).
-      assert (ENOTIN : ~E_t e) by apply ADD.
-      assert (MAPEQ : eq_dom E_t mapper' mapper).
-      { subst mapper'. unfolder. intros x XINE.
-        clear - ENOTIN XINE. rewrite updo.
-        all: congruence. }
-      assert (MAPER_E : mapper' ↑₁ eq e ≡₁ eq (ThreadEvent t_2 (index e - n))).
-      { subst mapper'. rewrite set_collect_eq. now rupd. }
-      assert (MAPSUB : mapper' ↑₁ E_t ≡₁ mapper ↑₁ E_t).
-      { clear - MAPEQ. now apply set_collect_eq_dom. }
-      assert (EQACTS : E_t' ≡₁ E_t ∪₁ eq e) by apply ADD.
-    
-      assert (NEWE :
-        << NINIT : ~is_init e >> /\
-        << NOTIN : ~E_s e >> /\
-        << TID : tid e = t_1 >>). 
-      { admit. }
-      unfold NW in NEWE. destruct NEWE as (NINIT & NOTIN & TID).
-      set (G_s' := {|
-        acts_set := E_s ∪₁ eq (ThreadEvent t_2 (index e - n));
-        threads_set := threads_set G_s;
-        lab := lab_t' ∘ mapper';
-        rf := mapper' ↑ rf_t';
-        co := mapper' ↑ co_t';
-        rmw := mapper' ↑ rmw_t';
-        rmw_dep := rmw_dep_t';
-        ctrl := ctrl_t';
-        data := data_t';
-        addr := addr_t';
-      |}).
-      set (X_s' := {|
-        WCore.sc := WCore.sc X_s;
-        WCore.G := G_s';
-      |}).
-      exists mapper', X_s'; splits.
-      { admit. }
-      { constructor; vauto; simpl; try basic_solver 6.
-        { rewrite (WCore.add_event_acts ADD). apply inj_dom_union.
-          { clear - SIMREL MAPEQ.
-            unfolder. ins. apply (seq_inj SIMREL); ins.
-            now rewrite <- !MAPEQ. }
-          { clear. basic_solver. }
-          rewrite MAPER_E, MAPSUB, (seq_codom SIMREL).
-          admit. }
-        { intros ev INE' TIDCOND.
-          destruct classic with (ev = e) as [EQ | NEQ].
-          { subst ev. unfold mapper'. rewrite upds; vauto.
-            unfold mapper' in TIDCOND. rewrite upds in TIDCOND; vauto. }
-          unfold mapper'. rewrite updo; vauto.
-          apply (seq_tid_1 SIMREL); vauto.
-          apply EQACTS in INE'. destruct INE' as [C1 | C2]; vauto.
-          unfold mapper' in TIDCOND. rewrite updo in TIDCOND; vauto. }
-        { intros ev INE' TIDCOND.
-          destruct classic with (ev = e) as [EQ | NEQ]; vauto.
-          { rewrite EQ; vauto. }
-          apply (seq_tid_2 SIMREL); vauto.
-          { apply EQACTS in INE'. destruct INE' as [C1 | C2]; vauto.
-            exfalso; basic_solver. }
-          unfold mapper' in TIDCOND.
-          rewrite updo in TIDCOND; vauto. }
-        { unfold compose.
-        
-        rewrite (WCore.add_event_acts ADD).
-          rewrite eq_dom_union; splits.
-          { destruct SIMREL. unfold mapper'.
-            intros x COND. unfold compose.
-            rewrite updo.
-            { apply seq_tid_4; auto. }
-            intros EQ. basic_solver. }
-          intros x COND. unfold compose.
-          unfold mapper'; subst. rewrite upds.
-          admit. }
-        { intros x COND. unfold compose. unfold mapper'.
-          destruct classic with (x = e) as [EQ | NEQ].
-          { admit. }
-          admit. }
-        { admit. }
-        all : admit. }
-      constructor.
-      { unfold WCore.add_event.
-        exists (option_map mapper' r), (mapper' ↑₁ R1),
-            (option_map mapper' w),
-            (mapper' ↑₁ W1),
-            (mapper' ↑₁ W2).
-        apply add_event_to_wf; simpl; vauto.
-        { apply sico_init_acts_s with
-                (X_t := X_t) (mapper := mapper).
-          { constructor. all : admit. }
-          destruct ADD. apply add_event_init. }
-        { unfold mapper'. rewrite upds. admit. }
-        { unfold mapper'. rewrite upds; vauto. }
-        { unfold mapper'. rewrite upds. basic_solver. }
-        { clear - MAPER_E. admit. }
-        
-        { unfold mapper'. rewrite upds.
-          destruct ADD; vauto. }
-        all : admit. }
-      all : admit. } }
-    
-      set (mapper' := upd mapper e e).
+  set (G_s' := {|
+    acts_set := E_s ∪₁ eq (ThreadEvent t_2 (index e - n));
+    threads_set := threads_set G_s;
+    lab := lab_t' ∘ mapper';
+    rf := mapper' ↑ rf_t';
+    co := mapper' ↑ co_t';
+    rmw := mapper' ↑ rmw_t';
+    rmw_dep := rmw_dep_t';
+    ctrl := ctrl_t';
+    data := data_t';
+    addr := addr_t';
+  |}).
+  set (X_s' := {|
+    WCore.sc := WCore.sc X_s;
+    WCore.G := G_s';
+  |}).
 
-      assert (ENOTIN : ~E_t e) by apply ADD.
-      assert (MAPEQ : eq_dom E_t mapper' mapper).
-      { subst mapper'. unfolder. intros x XINE.
-        clear - ENOTIN XINE. rewrite updo.
-        all: congruence. }
-      assert (MAPER_E : mapper' ↑₁ eq e ≡₁ eq e).
-      { subst mapper'. rewrite set_collect_eq. now rupd. }
-      assert (MAPSUB : mapper' ↑₁ E_t ≡₁ mapper ↑₁ E_t).
-      { clear - MAPEQ. now apply set_collect_eq_dom. }
-      assert (EQACTS : E_t' ≡₁ E_t ∪₁ eq e) by apply ADD.
+  exists mapper', X_s'; splits.
+  { admit. }
+  { constructor; vauto; simpl; try basic_solver 6.
+    { rewrite (WCore.add_event_acts ADD). apply inj_dom_union.
+      { clear - SIMREL MAPEQ.
+        unfolder. ins. apply (seq_inj SIMREL); ins.
+        now rewrite <- !MAPEQ. }
+      { clear. basic_solver. }
+      rewrite MAPER_E, MAPSUB, (seq_codom SIMREL).
+      admit. }
+    { intros ev INE' TIDCOND.
+      destruct classic with (ev = e) as [EQ | NEQ].
+      { subst ev. unfold mapper'. rewrite upds; vauto.
+        unfold mapper' in TIDCOND. rewrite upds in TIDCOND; vauto. }
+      unfold mapper'. rewrite updo; vauto.
+      apply (seq_tid_1 SIMREL); vauto.
+      apply EQACTS in INE'. destruct INE' as [C1 | C2]; vauto.
+      unfold mapper' in TIDCOND. rewrite updo in TIDCOND; vauto. }
+    { intros ev INE' TIDCOND.
+      destruct classic with (ev = e) as [EQ | NEQ]; vauto.
+      { rewrite EQ; vauto. }
+      apply (seq_tid_2 SIMREL); vauto.
+      { apply EQACTS in INE'. destruct INE' as [C1 | C2]; vauto.
+        exfalso; basic_solver. }
+      unfold mapper' in TIDCOND.
+      rewrite updo in TIDCOND; vauto. }
+    { unfold compose.
+      admit. }
+    { admit. }
+    { admit. }
+    all : admit. }
+  constructor.
+  { unfold WCore.add_event.
+    exists (option_map mapper' r), (mapper' ↑₁ R1),
+        (option_map mapper' w),
+        (mapper' ↑₁ W1),
+        (mapper' ↑₁ W2).
+    apply add_event_to_wf; simpl; vauto.
+    { apply sico_init_acts_s with
+            (X_t := X_t) (mapper := mapper).
+      { constructor. all : admit. }
+      destruct ADD. apply add_event_init. }
+    { unfold mapper'. rewrite upds. admit. }
+    { unfold mapper'. rewrite upds; vauto. }
+    { unfold mapper'. rewrite upds. basic_solver. }
+    { clear - MAPER_E. admit. }
+    { unfold mapper'. rewrite upds.
+      destruct ADD; vauto. }
+    all : admit. }
+  all : admit. 
+Admitted.
 
-      assert (NEWE :
-      << NINIT : ~is_init e >> /\
-      << NOTIN : ~E_s e >> /\
-      << TID : tid e = t_1 >>).
-      { admit. }
-      unfold NW in NEWE. destruct NEWE as (NINIT & NOTIN & TID).
+Lemma simrel_step_e_else
+    (T1 : tid e <> t_1)
+    (NINIT1 : t_1 <> tid_init)
+    (NINIT2 : t_2 <> tid_init)
+    (T2NOTIN : ~ threads_set G_t t_2)
+    (THRDNEQ : t_1 <> t_2)
+    (SIMREL : seq_simrel X_s X_t t_1 t_2 mapper)
+    (STEP : WCore.exec_inst X_t X_t' e l)
+    (MAPINV : eq_dom E_t (mapper ∘ mapper) id) :
+  exists mapper' X_s',
+    << MAPINV' : eq_dom E_t' (mapper' ∘ mapper') id >> /\
+    << SIMREL : seq_simrel X_s' X_t' t_1 t_2 mapper' >> /\
+    << STEP : WCore.exec_inst X_s X_s' (mapper' e) l >>.
+Proof using.
+  destruct STEP as [ADD RFC CONS].
+  destruct ADD as (r & R1 & w & W1 & W2 & ADD).
+  set (mapper' := upd mapper e e).
+  assert (ENOTIN : ~E_t e) by apply ADD.
+  assert (MAPEQ : eq_dom E_t mapper' mapper).
+  { subst mapper'. unfolder. intros x XINE.
+    clear - ENOTIN XINE. rewrite updo.
+    all: congruence. }
+  assert (MAPER_E : mapper' ↑₁ eq e ≡₁ eq e).
+  { subst mapper'. rewrite set_collect_eq. now rupd. }
+  assert (MAPSUB : mapper' ↑₁ E_t ≡₁ mapper ↑₁ E_t).
+  { clear - MAPEQ. now apply set_collect_eq_dom. }
+  assert (EQACTS : E_t' ≡₁ E_t ∪₁ eq e) by apply ADD.
+  assert (NEWE :
+  << NINIT : ~is_init e >> /\
+  << NOTIN : ~E_s e >> /\
+  << TID : tid e = t_1 >>).
+  { admit. }
+  unfold NW in NEWE. destruct NEWE as (NINIT & NOTIN & TID).
 
-      set (G_s' := {|
-      acts_set := mapper' ↑₁ E_t';
-        threads_set := threads_set G_s;
-        lab := lab_t' ∘ mapper';
-        rf := mapper' ↑ rf_t';
-        co := mapper' ↑ co_t';
-        rmw := mapper' ↑ rmw_t';
-        rmw_dep := rmw_dep_t';
-        ctrl := ctrl_t';
-        data := data_t';
-        addr := addr_t';
-      |}).
-      set (X_s' := {|
-        WCore.sc := WCore.sc X_s;
-        WCore.G := G_s';
-      |}).
+  set (G_s' := {|
+  acts_set := mapper' ↑₁ E_t';
+    threads_set := threads_set G_s;
+    lab := lab_t' ∘ mapper';
+    rf := mapper' ↑ rf_t';
+    co := mapper' ↑ co_t';
+    rmw := mapper' ↑ rmw_t';
+    rmw_dep := rmw_dep_t';
+    ctrl := ctrl_t';
+    data := data_t';
+    addr := addr_t';
+  |}).
+  set (X_s' := {|
+    WCore.sc := WCore.sc X_s;
+    WCore.G := G_s';
+  |}).
 
-      exists mapper', X_s'; splits.
-      { admit. }
-      { constructor; vauto; simpl; try basic_solver 6. }
-       
-      constructor.
-      { unfold WCore.add_event.
-        exists (option_map mapper' r), (mapper' ↑₁ R1),
-            (option_map mapper' w),
-            (mapper' ↑₁ W1),
-            (mapper' ↑₁ W2).
-        apply add_event_to_wf; simpl; vauto. }
-      all : admit. 
-
+  exists mapper', X_s'; splits.
+  { admit. }
+  { constructor; vauto; simpl; try basic_solver 6. }
+  constructor.
+  { unfold WCore.add_event.
+    exists (option_map mapper' r), (mapper' ↑₁ R1),
+        (option_map mapper' w),
+        (mapper' ↑₁ W1),
+        (mapper' ↑₁ W2).
+    apply add_event_to_wf; simpl; vauto. }
+  all : admit. 
 Admitted.
 
 Definition seq_graph_rex : execution := {|
@@ -810,3 +832,49 @@ Proof using.
 Admitted.
 
 End SimrelMain.
+
+Section ProgMain.
+
+Variable X_t : WCore.t.
+Variable t_1 t_2 : thread_id.
+Variable threads : thread_id -> Prop.
+
+Variable p1 p2 : program.
+
+Definition X_t_init : WCore.t := WCore.Build_t (WCore.init_exec threads) ∅₂.
+Definition X_s_init : WCore.t := WCore.Build_t (WCore.init_exec (threads ∪₁ eq t_2)) ∅₂.
+
+Hypothesis PROGSEQ : program_sequented p1 p2 t_1 t_2.
+
+Lemma prog_supp : 
+  exists X_s mapper,
+    << SIMREL : seq_simrel X_s X_t t_1 t_2 mapper >> /\
+    << STEP   : xmm_step＊ X_s_init X_s >> /\
+    << BEHRS  : same_behaviors (WCore.G X_s) (WCore.G X_t) >>.
+Proof using.
+  admit.
+Admitted.
+
+Lemma prog_helper X_s mapper :
+  seq_simrel X_s X_t t_1 t_2 mapper ->
+  exec_sequent X_s X_t p1 p2 t_1 t_2.
+Proof using.
+  intros SIMREL.
+  constructor; vauto.
+  intros tr_1 tr2 TR1 TR2 CR1 CR2.
+  constructor. all : admit.
+Admitted.
+
+Lemma prog_main :
+  exists X_s,
+    << SEQUED : exec_sequent X_s X_t p1 p2 t_1 t_2 >> /\
+    << STEP   : xmm_step＊ X_s_init X_s >> /\
+    << BEHRS  : same_behaviors (WCore.G X_s) (WCore.G X_t) >>.
+Proof using.
+  destruct prog_supp as (X_s & mapper & SIMREL & STEP & BEHRS).
+  exists X_s; splits; auto.
+  apply prog_helper with (mapper := mapper).
+  vauto.
+Qed.
+
+End ProgMain.
